theories/product.v
@@ -1,5 +1,6 @@
 Require Export refframe.module.
 Require Import refframe.srefines.
+Require Import refframe.trefines.
 Require Import refframe.filter.
 
 
@@ -24,9 +25,8 @@ Inductive product_step {EV1 EV2} (m1 : module EV1) (m2 : module EV2) :
                  (λ '(σ1', σ2'), Pσ1 σ1' ∧ Pσ2 σ2')
 .
 
-Definition mod_product {EV1 EV2} (m1 : module EV1) (m2 : module EV2) : module (option EV1 * option EV2) := {|
-  m_step := product_step m1 m2;
-|}.
+Definition mod_product {EV1 EV2} (m1 : module EV1) (m2 : module EV2) : module (option EV1 * option EV2) :=
+  Mod (product_step m1 m2).
 
 Module test3.
 
@@ -130,9 +130,7 @@ Inductive prod_mod1_step : nat → option nat → (nat → Prop) → Prop :=
 | PM1S5: prod_mod1_step 5 (Some 4) (λ σ', σ' = 6)
 .
 
-Definition prod_mod1 : module nat := {|
-  m_step := prod_mod1_step;
-|}.
+Definition prod_mod1 : module nat := Mod prod_mod1_step.
 
 Inductive prod_modA_step : nat → option nat → (nat → Prop) → Prop :=
 | PMAS0 : prod_modA_step 0 (Some 10) (λ σ', σ' = 1)
@@ -144,9 +142,7 @@ Inductive prod_modA_step : nat → option nat → (nat → Prop) → Prop :=
 | PMAS6 : prod_modA_step 6 (Some 11) (λ σ', σ' = 7)
 .
 
-Definition prod_modA : module nat := {|
-  m_step := prod_modA_step;
-|}.
+Definition prod_modA : module nat := Mod prod_modA_step.
 
 Inductive prod_modB_step : nat → option nat → (nat → Prop) → Prop :=
 | PMBS0: prod_modB_step 0 None (λ σ', σ' = 1 ∨ σ' = 5)
@@ -158,9 +154,7 @@ Inductive prod_modB_step : nat → option nat → (nat → Prop) → Prop :=
 | PMBS7: prod_modB_step 7 (Some 4) (λ σ', σ' = 8)
 .
 
-Definition prod_modB : module nat := {|
-  m_step := prod_modB_step;
-|}.
+Definition prod_modB : module nat := Mod prod_modB_step.
 
 Inductive prod_modB'_step : nat → option nat → (nat → Prop) → Prop :=
 | PMB'S0: prod_modB'_step 0 (Some 10) (λ σ', σ' = 1)
@@ -170,9 +164,7 @@ Inductive prod_modB'_step : nat → option nat → (nat → Prop) → Prop :=
 | PMB'S5: prod_modB'_step 5 (Some 4) (λ σ', σ' = 6)
 .
 
-Definition prod_modB' : module nat := {|
-  m_step := prod_modB'_step;
-|}.
+Definition prod_modB' : module nat := Mod (prod_modB'_step).
 
 Definition filterR (e1 : (option nat * option nat)) (e2 : option nat) : Prop :=
     (e1 = (Some 10, Some 10) ∧ e2 = None)
@@ -357,3 +349,454 @@ Proof.
            split. admit.
            move => [??].
 Admitted.
+
+(*** trefines for [product] *)
+Inductive mod_product_rel {EV1 EV2} : trace (option EV1 * option EV2) → trace EV1 → trace EV2 → Prop :=
+| MPR_nil κs :
+    tnil ⊆ κs →
+    mod_product_rel κs tnil tnil
+| MPR_ex1 T f κs κs2 :
+    (∀ x, mod_product_rel κs (f x) κs2) →
+    mod_product_rel κs (tex T f) κs2
+| MPR_ex2 T f κs κs2 :
+    (∀ x, mod_product_rel κs κs2 (f x)) →
+    mod_product_rel κs κs2 (tex T f)
+| MPR_all1 {T} x f κs κs2 :
+    mod_product_rel κs (f x) κs2 →
+    mod_product_rel κs (tall T f) κs2
+| MPR_all2 {T} x f κs κs2 :
+    mod_product_rel κs κs2 (f x) →
+    mod_product_rel κs κs2 (tall T f)
+| MPR_all T f κs κs1 κs2:
+    (∀ x, mod_product_rel (f x) κs1 κs2) →
+    (tall T f) ⊆ κs →
+    mod_product_rel κs κs1 κs2
+| MPR_cons_l κ κs κs' κs1' κs2 :
+    mod_product_rel κs' κs1' κs2 →
+    tcons (Some κ, None) κs' ⊆ κs →
+    mod_product_rel κs (tcons κ κs1') κs2
+| MPR_cons_r κ κs κs' κs1 κs2' :
+    mod_product_rel κs' κs1 κs2' →
+    tcons (None, Some κ) κs' ⊆ κs →
+    mod_product_rel κs κs1 (tcons κ κs2')
+| MPR_cons_both κ1 κ2 κs κs' κs1' κs2' :
+    mod_product_rel κs' κs1' κs2' →
+    tcons (Some κ1, Some κ2) κs' ⊆ κs →
+    mod_product_rel κs (tcons κ1 κs1') (tcons κ2 κs2')
+.
+
+
+Lemma mod_product_rel_mono {EV1 EV2} κs κs' (κs1 : trace EV1) (κs2 : trace EV2) :
+  mod_product_rel κs κs1 κs2 →
+  κs ⊆ κs' →
+  mod_product_rel κs' κs1 κs2.
+Proof.
+  move => Ht.
+  elim: Ht κs'.
+  - move => ????. constructor. by etrans.
+  - move => *. constructor. naive_solver.
+  - move => *. constructor. naive_solver.
+  - move => *. econstructor. naive_solver.
+  - move => *. econstructor; naive_solver.
+  - move => *. eapply MPR_all. 2: by etrans. naive_solver.
+  - move => ????? ?? IH ??.
+    apply: MPR_cons_l; [| by etrans]. naive_solver.
+  - move => ????? ?? IH ??.
+    apply: MPR_cons_r; [| by etrans]. naive_solver.
+  - move => *.
+    apply: MPR_cons_both; [| by etrans]. naive_solver.
+Qed.
+
+
+Lemma tmod_product_to_mods {EV1 EV2} (m1 : module EV1) (m2 : module EV2) σ Pσ κs:
+  σ ~{ mod_product m1 m2, κs }~>ₜ Pσ → ∃ κs', mod_product_rel κs κs'.1 κs'.2 ∧
+    σ.1 ~{ m1, κs'.1 }~>ₜ (λ _, True) ∧ σ.2 ~{ m2, κs'.2 }~>ₜ (λ _, True).
+Proof.
+  elim.
+  - move => [σ1 σ2] ????. eexists (tnil, tnil) => /=.
+    split_and!.
+    + apply: mod_product_rel_mono; [|done]. by constructor.
+    + by constructor.
+    + by constructor.
+  - move => [σ1 σ2] ????? Hstep _ IH ?.
+    inversion Hstep; simplify_eq.
+    + have {}IH := IH (_, σ2) (conj _ ltac:(exact (eq_refl σ2))).
+      have [f Hf]:= CHOICE IH.
+      unshelve eexists (tapp (option_trace e) (tex _ (λ x, (f x).1)), (tall _ (λ x, (f x).2))) => /=.
+      split_and!.
+      -- apply: mod_product_rel_mono; [|done].
+         destruct e => //=.
+         ++ apply: MPR_cons_l; [|done].
+            constructor => -[??]. econstructor.
+            naive_solver.
+         ++ constructor => -[??]. econstructor. naive_solver.
+      -- apply: TTraceStep; [ done | | done].
+         move => σ' Hσ'. apply: (thas_trace_ex (exist _ σ' Hσ')).
+         apply: thas_trace_mono. naive_solver. done. naive_solver.
+      -- apply: thas_trace_all => -[??].
+         apply: thas_trace_mono. naive_solver. done. naive_solver.
+    + have {}IH := IH (σ1, _) (conj ltac:(exact (eq_refl σ1)) _).
+      have [f Hf]:= CHOICE IH.
+      unshelve eexists ((tall _ (λ x, (f x).1)), tapp (option_trace e) (tex _ (λ x, (f x).2))) => /=.
+      split_and!.
+      -- apply: mod_product_rel_mono; [|done].
+         destruct e => //=.
+         ++ apply: MPR_cons_r; [|done].
+            constructor => -[??]. econstructor.
+            naive_solver.
+         ++ constructor => -[??]. econstructor. naive_solver.
+      -- apply: thas_trace_all => -[??].
+         apply: thas_trace_mono. naive_solver. done. naive_solver.
+      -- apply: TTraceStep; [ done | | done].
+         move => σ' Hσ'. apply: (thas_trace_ex (exist _ σ' Hσ')).
+         apply: thas_trace_mono. naive_solver. done. naive_solver.
+    + have {}IH := IH (_, _) (conj _ _).
+      have [f Hf]:= CHOICE2 IH.
+      unshelve eexists (tcons e1 (tex _ (λ x1, (tall _ (λ x2, (f x1 x2).1)))),
+                        tcons e2 (tex _ (λ x2, (tall _ (λ x1, (f x1 x2).2))))) => /=.
+      split_and!.
+      -- apply: mod_product_rel_mono; [|done]. simpl.
+         econstructor; [|done..].
+         constructor => -[??].
+         constructor => -[??].
+         econstructor.
+         econstructor. naive_solver.
+      -- apply: TTraceStep; [ done | | simpl; done].
+         move => ??.
+         apply: thas_trace_ex. apply: thas_trace_all => -[??]. naive_solver.
+      -- apply: TTraceStep; [ done | | simpl; done].
+         move => ??.
+         apply: thas_trace_ex. apply: thas_trace_all => -[??]. naive_solver.
+  - move => T f ???? IH ?.
+    have [fx Hfx]:= AxCHOICE _ _ _ IH.
+    eexists (tall T (λ x, (fx x).1), tall T (λ x, (fx x).2)) => /=.
+    split_and! => //.
+    -- apply: mod_product_rel_mono; [|done].
+       eapply MPR_all; [|done] => ?.
+       econstructor. econstructor. naive_solver.
+    -- apply: thas_trace_all. naive_solver.
+    -- apply: thas_trace_all. naive_solver.
+       Unshelve. done. done.
+Qed.
+
+Lemma mod_product_nil_l {EV1 EV2} (m1 : module EV1) (m2 : module EV2) σ1 σ2 Pσ κs:
+  σ1 ~{ m1, κs }~>ₜ Pσ → κs ⊆ tnil →
+  (σ1, σ2) ~{ mod_product m1 m2, tnil }~>ₜ (λ σ', Pσ σ'.1 ∧ σ2 = σ'.2).
+Proof.
+  elim.
+  - move => ??????. constructor; [|done]. naive_solver.
+  - move => ??? κ ????? Hs1 Hs2.
+    pose proof (transitivity Hs1 Hs2) as Hs.
+    destruct κ; [inversion Hs|]; simplify_eq/=.
+    apply: TTraceStep; [ by apply: ProductStepL | | simpl;done].
+    move => [??] /=. naive_solver.
+  - move => ??????? Hs1 Hs2.
+    pose proof (transitivity Hs1 Hs2) as [??]%subtrace_all_nil_inv. naive_solver.
+Qed.
+
+Lemma mod_product_nil_r {EV1 EV2} (m1 : module EV1) (m2 : module EV2) σ1 σ2 Pσ κs:
+  σ2 ~{ m2, κs }~>ₜ Pσ → κs ⊆ tnil →
+  (σ1, σ2) ~{ mod_product m1 m2, tnil }~>ₜ (λ σ', Pσ σ'.2 ∧ σ1 = σ'.1).
+Proof.
+  elim.
+  - move => ??????. constructor; [|done]. naive_solver.
+  - move => ??? κ ????? Hs1 Hs2.
+    pose proof (transitivity Hs1 Hs2) as Hs.
+    destruct κ; [inversion Hs|]; simplify_eq/=.
+    apply: TTraceStep; [ by apply: ProductStepR | | simpl;done].
+    move => [??] /=. naive_solver.
+  - move => ??????? Hs1 Hs2.
+    pose proof (transitivity Hs1 Hs2) as [??]%subtrace_all_nil_inv. naive_solver.
+Qed.
+
+Lemma tmods_to_mod_product {EV1 EV2} (m1 : module EV1) (m2 : module EV2) σ κs κs1 κs2:
+  mod_product_rel κs κs1 κs2 →
+  σ.1 ~{ m1, κs1 }~>ₜ (λ _, True) → σ.2 ~{ m2, κs2 }~>ₜ (λ _, True) →
+  σ ~{ mod_product m1 m2, κs }~>ₜ (λ _, True).
+Proof.
+  move => Hrel.
+  elim: Hrel σ.
+  - move => ?????. by constructor.
+  - move => ????? /= IH [??] /thas_trace_ex_inv ??.
+    apply: (thas_trace_trans tnil). { by apply: mod_product_nil_l. }
+    move => [??] /= [[??]?]. naive_solver.
+  - move => ????? IH [??] ? /thas_trace_ex_inv ?.
+    apply: (thas_trace_trans tnil). { by apply: mod_product_nil_r. }
+    move => [??] /= [[??]?]. naive_solver.
+  - move => ?????? IH ? /thas_trace_all_inv ??. apply: IH; [|done]. naive_solver.
+  - move => ?????? IH ?? /thas_trace_all_inv ?. apply: IH; [done|]. naive_solver.
+  - move => ?????? IH ????.
+    apply: thas_trace_mono; [|done| done].
+    apply: thas_trace_all => ?. naive_solver.
+  - move => ?????? IH ? [??]/= /(thas_trace_cons_inv _ _) ??.
+    apply: thas_trace_mono; [|done| done].
+    apply: (thas_trace_trans tnil). { by apply: mod_product_nil_l. }
+    move => /= [??] /= [[?[??]]?]. subst.
+    apply: TTraceStep; [ by apply: ProductStepL |  | simpl;done].
+    move => [??] /= [??]. subst. naive_solver.
+  - move => ?????? IH ? [??]/=? /(thas_trace_cons_inv _ _)?.
+    apply: thas_trace_mono; [|done| done].
+    apply: (thas_trace_trans tnil). { by apply: mod_product_nil_r. }
+    move => /= [??] /= [[?[??]]?]. subst.
+    apply: TTraceStep; [ by apply: ProductStepR |  | simpl;done].
+    move => [??] /= [??]. subst. naive_solver.
+  - move => ??????? IH ? [??]/= /(thas_trace_cons_inv _ _)? /(thas_trace_cons_inv _ _)?.
+    apply: thas_trace_mono; [|done| done].
+    apply: (thas_trace_trans tnil). { by apply: mod_product_nil_l. }
+    move => /= [??] /= [[?[??]]?]. subst.
+    apply: (thas_trace_trans tnil). { by apply: mod_product_nil_r. }
+    move => /= [??] /= [[?[??]]?]. subst.
+    apply: TTraceStep; [ by apply: ProductStepBoth |  | simpl;done].
+    move => [??] /= [??]. subst. naive_solver.
+Qed.
+
+Lemma mod_product_trefines {EV1 EV2} (m1 m1' : module EV1) (m2 m2' : module EV2) σ1 σ1' σ2 σ2':
+  trefines (MS m1 σ1) (MS m1' σ1') →
+  trefines (MS m2 σ2) (MS m2' σ2') →
+  trefines (MS (mod_product m1 m2) (σ1, σ2)) (MS (mod_product m1' m2') (σ1', σ2')).
+Proof.
+  move => [/=Hr1] [/=Hr2]. constructor => κs /= /tmod_product_to_mods[κs1 [κs2 [/Hr1 ? /Hr2 ?]]].
+  by apply: tmods_to_mod_product.
+Qed.
+
+
+(*** Proving refinement *)
+
+(** ** [inv] *)
+Lemma inv_implies_trefines {EV} (m1 m2 : mod_state EV) (inv : m1.(m_state) → m2.(m_state) → Prop):
+  inv m1.(ms_state) m2.(ms_state) →
+  (∀ σi1 σs1 Pσi2 e,
+      inv σi1 σs1 → m_step m1 σi1 e Pσi2 →
+      σs1 ~{ m2, option_trace e }~>ₜ (λ σs2, ∃ σi2, Pσi2 σi2 ∧ inv σi2 σs2)) →
+  trefines m1 m2.
+Proof.
+  move => Hinvinit Hinvstep.
+  constructor => // κs. move: m1.(ms_state) m2.(ms_state) Hinvinit => σi1 σs1 Hinv Hsteps.
+  elim: Hsteps σs1 Hinv => {σi1 κs}.
+  - move => ???????. by constructor.
+  - move => σi1 Pσi2 Pσi3 κ κs κs' Hstep Hsteps IH Hcons σs1 Hinv.
+    have ?:= (Hinvstep _ _ _ _ Hinv Hstep).
+    apply: thas_trace_mono; [|done|done].
+    apply: thas_trace_trans; [done|] => ? /=[?[??]].
+    by apply: IH.
+  - move => ??????????.
+    apply: thas_trace_mono; [|done|done].
+    apply: thas_trace_all => ?. naive_solver.
+Qed.
+
+Lemma inv'_implies_trefines {EV} (m1 m2 : mod_state EV) (inv : m1.(m_state) → m2.(m_state) → trace EV → Prop):
+  (∀ κs, ms_state m1 ~{ m1, κs }~>ₜ (λ _, True) → inv m1.(ms_state) m2.(ms_state) κs) →
+  (∀ σi1 σs1 Pσi2 e κs κs',
+      inv σi1 σs1 κs → m_step m1 σi1 e Pσi2 → tapp (option_trace e) κs' ⊆ κs →
+      σs1 ~{ m2, option_trace e }~>ₜ (λ σs2, ∃ σi2, Pσi2 σi2 ∧ inv σi2 σs2 κs')) →
+  (∀ σi1 σs1 κs T f,
+      inv σi1 σs1 κs → tall T f ⊆ κs → ∀ x, inv σi1 σs1 (f x)) →
+  trefines m1 m2.
+Proof.
+  move => Hinvinit Hinvstep Hinvall.
+  constructor => // κs. move: m1.(ms_state) m2.(ms_state) (Hinvinit κs) => σi1 σs1 Hinv Hsteps.
+  move: (Hinv Hsteps) => {}Hinv.
+  elim: Hsteps σs1 Hinv => {σi1 κs}.
+  - move => ???????. by constructor.
+  - move => σi1 Pσi2 Pσi3 κ κs κs' Hstep Hsteps IH Hcons σs1 Hinv.
+    have ?:= (Hinvstep _ _ _ _ _ _ Hinv Hstep Hcons).
+    apply: thas_trace_mono; [|done|done].
+    apply: thas_trace_trans; [done|] => ? /=[?[??]].
+    by apply: IH.
+  - move => ?????? IH ???.
+    apply: thas_trace_mono; [|done|done].
+    apply: thas_trace_all => ?. naive_solver.
+Qed.
+
+Lemma trefines_implies_inv' {EV} (m1 m2 : mod_state EV):
+  trefines m1 m2 →
+  ∃ (inv : m1.(m_state) → m2.(m_state) → trace EV → Prop),
+  (∀ κs, ms_state m1 ~{ m1, κs }~>ₜ (λ _, True) → inv m1.(ms_state) m2.(ms_state) κs) ∧
+  (∀ σi1 σs1 Pσi2 e κs κs',
+      inv σi1 σs1 κs → m_step m1 σi1 e Pσi2 → tapp (option_trace e) κs' ⊆ κs →
+      σs1 ~{ m2, option_trace e }~>ₜ (λ σs2, ∃ σi2, Pσi2 σi2 ∧ inv σi2 σs2 κs')) ∧
+  (∀ σi1 σs1 κs T f,
+      inv σi1 σs1 κs → tall T f ⊆ κs → ∀ x, inv σi1 σs1 (f x)).
+Proof.
+  move => [Hr].
+  eexists (λ σi σs κs, σs ~{ m2, κs }~>ₜ (λ _, True)).
+  split_and!.
+  - done.
+  - move => {Hr} ?????????.  admit.
+  - admit.
+Abort.
+
+Lemma inv''_implies_trefines {EV} (m1 m2 : mod_state EV) (inv : m1.(m_state) → m2.(m_state) → trace EV → Prop):
+  (∀ κs, inv m1.(ms_state) m2.(ms_state) κs) →
+  (∀ σi1 σs1 Pσi2 e κs κs',
+      inv σi1 σs1 κs → m_step m1 σi1 e Pσi2 → tapp (option_trace e) κs' ⊆ κs →
+      σs1 ~{ m2, option_trace e }~>ₜ (λ σs2, ∃ σi2, Pσi2 σi2 ∧ inv σi2 σs2 κs')) →
+  (∀ σi1 σs1 κs T f,
+      inv σi1 σs1 κs → tall T f ⊆ κs → ∀ x, inv σi1 σs1 (f x)) →
+  trefines m1 m2.
+Proof. Abort.
+(*
+  move => Hinvinit Hinvstep Hinvall.
+  constructor => // κs. move: m1.(ms_state) m2.(ms_state) (Hinvinit κs) => σi1 σs1 Hinv Hsteps.
+  move: (Hinv Hsteps) => {}Hinv.
+  elim: Hsteps σs1 Hinv => {σi1 κs}.
+  - move => ???????. by constructor.
+  - move => σi1 Pσi2 Pσi3 κ κs κs' Hstep Hsteps IH Hcons σs1 Hinv.
+    have ?:= (Hinvstep _ _ _ _ _ _ Hinv Hstep Hcons).
+    apply: thas_trace_mono; [|done|done].
+    apply: thas_trace_trans; [done|] => ? /=[?[??]].
+    by apply: IH.
+  - move => ?????? IH ???.
+    apply: thas_trace_mono; [|done|done].
+    apply: thas_trace_all => ?. naive_solver.
+Qed.
+ *)
+(*
+Lemma trefines_implies_inv'' {EV} (m1 m2 : mod_state EV):
+  trefines m1 m2 →
+  ∃ (inv : m1.(m_state) → m2.(m_state) → trace EV → Prop),
+  (∀ κs, inv m1.(ms_state) m2.(ms_state) κs) ∧
+  (∀ σi1 σs1 Pσi2 e κs κs',
+      inv σi1 σs1 κs → m_step m1 σi1 e Pσi2 → tapp (option_trace e) κs' ⊆ κs →
+      σs1 ~{ m2, option_trace e }~>ₜ (λ σs2, ∃ σi2, Pσi2 σi2 ∧ inv σi2 σs2 κs')) ∧
+  (∀ σi1 σs1 κs T f,
+      inv σi1 σs1 κs → tall T f ⊆ κs → ∀ x, inv σi1 σs1 (f x)).
+Proof.
+  move => [Hr].
+  eexists (λ σi σs κs, σs ~{ m2, κs }~>ₜ (λ _, True)).
+  split_and!.
+  - done.
+  - move => {Hr} ?????????.  admit.
+  - admit.
+Abort.
+*)
+
+Lemma forall_to_ex1 A B (P1 : A → Prop)  P2 (Q : B → Prop):
+ (∃ n : A, P1 n ∧ (∀ y, P2 n y → Q y)) -> (∀ y, (∀ n : A, P1 n → P2 n y) → Q y).
+Proof. naive_solver. Qed.
+
+Lemma trefines_implies_trefines {EV} (m1 m2 : mod_state EV):
+  trefines m1 m2 → trefines m1 m2.
+Proof.
+  move => [/=Hr]. constructor => κs Ht.
+  move: Hr. move: (ms_state m1) (ms_state m2) Ht => σ1 σ2 Ht.
+  move: σ2. apply: forall_to_ex1.
+  elim: Ht.
+  - move => ?????. eexists tnil. split; [ by apply: TTraceEnd|]. move => ??. by apply: TTraceEnd.
+  - move => ??? κ ?? Hstep ? IH ?.
+    have [f Hf]:= CHOICE IH.
+    eexists (tapp (option_trace κ) (tex _ f)). split.
+    + apply: TTraceStep; [done| |done]. move => ??. apply: thas_trace_ex. naive_solver.
+    + move => σ2. destruct κ; simplify_eq/=.
+      * move => /(thas_trace_cons_inv _ _) Ht.
+        apply: (thas_trace_trans tnil); [done|] => ? [?[? {}Ht]].
+        apply: thas_trace_mono; [|done|done].
+        apply: TTraceStep; [done | |simpl; done]. move => ??.
+        have /thas_trace_ex_inv{}Ht := Ht _ ltac:(done).
+        apply: (thas_trace_trans tnil); [done|] => ? [[??]?].
+        apply: thas_trace_mono; [|done| ]. naive_solver. done.
+      * move => /thas_trace_ex_inv Ht.
+        apply: (thas_trace_trans tnil); [done|] => ? [[??]?].
+        apply: thas_trace_mono; [|done|done]. naive_solver.
+  - move => ?????? IH ?.
+    have [fx Hfx]:= AxCHOICE _ _ _ IH.
+    eexists (tall _ (λ x, fx x)). split.
+    + apply: thas_trace_all. naive_solver.
+    + move => ? /thas_trace_all_inv ?. apply: thas_trace_mono; [|done|done].
+      apply: thas_trace_all. naive_solver.
+      Unshelve. done.
+Qed.
+
+Lemma forall_to_ex2 A B1 B2 (P1 : A → Prop)  P2 (Q : B1 → B2 → Prop) R:
+ (∃ n : A, P1 n ∧ (∀ y1 y2, R y1 y2 → P2 n y1 y2 → Q y1 y2)) -> (∀ y1 y2, R y1 y2 → (∀ n : A, P1 n → P2 n y1 y2) → Q y1 y2).
+Proof. naive_solver. Qed.
+
+Lemma trefines1_implies_trefines2 {EV1 EV2} (mi1 ms1 : mod_state EV1) (mi2 ms2 : mod_state EV2)
+      (iinv : mi1.(m_state) → mi2.(m_state) → Prop)
+      (sinv : ms1.(m_state) → ms2.(m_state) → Prop):
+  trefines mi1 ms1 →
+  iinv mi1.(ms_state) mi2.(ms_state) →
+  sinv ms1.(ms_state) ms2.(ms_state) →
+  (∀ σ1 σ2 κ Pσ2, iinv σ1 σ2 → m_step mi2 σ2 κ Pσ2 → ∃ κ',
+    (if κ' is Some e then
+       ∀ σs1 σs2 Pσs1, sinv σs1 σs2 → m_step ms1 σs1 κ' Pσs1 →
+          σs2 ~{ ms2, option_trace κ }~>ₜ (λ σs2', ∃ σs1', Pσs1 σs1' ∧ sinv σs1' σs2')
+     else κ = None) ∧
+       σ1 ~{ mi1, option_trace κ' }~>ₜ (λ σ1', ∃ σ2', Pσ2 σ2' ∧ iinv σ1' σ2')) →
+  (∀ σ1 σ2 Pσ1, sinv σ1 σ2 → m_step ms1 σ1 None Pσ1 →
+                σ2 ~{ ms2, tnil }~>ₜ (λ σ2', ∃ σ1', Pσ1 σ1' ∧ sinv σ1' σ2')) →
+  trefines mi2 ms2.
+Proof.
+  move => [/=Hr] Hiinvinit Hsinvinit Histep Hsnil.
+  have {}Hsnil: (∀ σ1 σ2 Pσ1, sinv σ1 σ2 → σ1 ~{ ms1, tnil }~>ₜ Pσ1 →
+                σ2 ~{ ms2, tnil }~>ₜ (λ σ2', ∃ σ1', Pσ1 σ1' ∧ sinv σ1' σ2')). {
+    clear -Hsnil.
+    move => σ1 σ2 Pσ1 Hsinv /thas_trace_nil_inv.
+    have : @tnil EV1 ⊆ tnil by done. move: {1 3}(@tnil EV1) => κs Hκs Ht.
+    elim: Ht σ2 Hsinv Hκs.
+    - move => ????????. apply: TTraceEnd; naive_solver.
+    - move => ??? κ ?? Hstep ? IH Hs1 ?? Hs2.
+      pose proof (transitivity Hs1 Hs2) as Hs. destruct κ; simplify_eq/=; [easy| ].
+      move: Hstep => /Hsnil {}Hstep.
+      apply: (thas_trace_trans tnil); naive_solver.
+  }
+  constructor => κs Ht. move: Hiinvinit Hsinvinit Hr.
+  move: (ms_state mi1) (ms_state mi2) (ms_state ms1) (ms_state ms2) Ht => σi1 σi2 σs1 σs2 Ht Hiinit Hsinit.
+  move: σs1 σs2 Hsinit. apply: forall_to_ex2.
+  elim: Ht σi1 Hiinit.
+  - move => ???????. eexists tnil. split; [ by apply: TTraceEnd|]. move => ????. by apply: TTraceEnd.
+  - move => ? Pσ2 ? κ ? κs' Hstep ? IH ? ? Hiinv.
+    have [κ' [Hsend Hsteps]]:= Histep _ _ _ _ Hiinv Hstep.
+    have {}IH : ∀ σi1, (∃ σ2', Pσ2 σ2' ∧ iinv σi1 σ2') → ∃ n, σi1 ~{ mi1, n }~>ₜ (λ _, True) ∧
+       (∀ y1 y2, sinv y1 y2 → y1 ~{ ms1, n }~>ₜ (λ _, True) → y2 ~{ ms2, κs' }~>ₜ (λ _, True)).
+    { move => ?. naive_solver. }
+    have [f Hf]:= CHOICE IH.
+    eexists (tapp (option_trace κ') (tex _ f)). split.
+    + apply: thas_trace_trans; [done| ] => ?[?[??]].
+      apply: thas_trace_ex. naive_solver.
+    + move => σs1 σs2 ? /thas_trace_app_inv Happ.
+      apply: (thas_trace_mono _ _ (λ _, True)); [|done|done].
+      move: Happ. destruct κ'; simplify_eq/=.
+      * move => /(thas_trace_cons_inv _ _)/Hsnil Ht.
+        apply: (thas_trace_trans tnil); [naive_solver|].
+        move => {Ht} ? [? [[?[? HP]]?]].
+        apply: thas_trace_trans; [naive_solver|].
+        move => ?[?[??]].
+        have /Hsnil ?:= HP _ ltac:(done).
+        apply: (thas_trace_trans tnil); [naive_solver|].
+        move => ? [?[/thas_trace_ex_inv/Hsnil??]].
+        apply: (thas_trace_trans tnil); [naive_solver|].
+        move => ?[?[[[?[?[??]]]?]?]].
+        naive_solver.
+      * move => /Hsnil Hs.
+        apply: (thas_trace_trans tnil); [naive_solver|].
+        move => ? [? [/thas_trace_ex_inv/Hsnil? ?]].
+        apply: (thas_trace_trans tnil); [naive_solver|].
+        move => ? [?[[[?[?[??]]]?]?]]. naive_solver.
+  - move => ?????? IH ???.
+    have {}IH := (IH _ _ ltac:(done)).
+    have [fx Hfx]:= AxCHOICE _ _ _ IH.
+    eexists (tall _ (λ x, fx x)). split.
+    + apply: thas_trace_all. naive_solver.
+    + move => ??? /thas_trace_all_inv ?. apply: thas_trace_mono; [|done|done].
+      apply: thas_trace_all. naive_solver.
+      Unshelve. all: naive_solver.
+Qed.
+
+Lemma tmod_filter_refines' {EV1 EV2} (R : EV1 → option EV2 → Prop) mi ms σi σs:
+  trefines (MS mi σi) (MS ms σs) →
+  trefines (MS (mod_filter mi R) σi) (MS (mod_filter ms R) σs).
+Proof.
+  move => Hr. eapply (trefines1_implies_trefines2 (MS mi _) (MS ms _) (MS (mod_filter mi R) _) (MS (mod_filter ms R) _) (λ σ1 σ2, σ1 = σ2) (λ σ1 σ2, σ1 = σ2)); [done.. | |] => /=.
+  - move => ???? -> Hstep. inversion Hstep; simplify_eq. eexists e.
+    split.
+    + case_match; simplify_eq => //.
+      move => ??? -> ?. apply: TTraceStep; [| |by erewrite tapp_tnil_r].
+      { econstructor; [done| simpl; done]. }
+      move => ??. apply: TTraceEnd; naive_solver.
+    + apply: TTraceStep; [done| |by erewrite tapp_tnil_r].
+      move => ??. apply: TTraceEnd; [|done]. naive_solver.
+  - move => ??? -> ?.
+    apply: TTraceStep; [by econstructor| |simpl; done].
+    move => ??. apply: TTraceEnd; [|done]. naive_solver.
+Qed.
