theories/refines_meta.v
@@ -1,0 +1,322 @@
+Require Export refframe.module.
+Require Import refframe.srefines.
+Require Import refframe.trefines.
+Require Import refframe.dem_module.
+Require Import refframe.example_modules.
+
+(*** Proof that trefines implies srefines *)
+Inductive thas_trace_rel {EV} : (list (event EV) → Prop) → (trace EV) → Prop :=
+| TRel_nil (Pκs : _ → Prop) κs:
+   κs ⊆ tnil →
+   Pκs [] →
+   Pκs [Nb] →
+   thas_trace_rel Pκs κs
+| TRel_cons (Pκs : _ → Prop) κ κs κs':
+   κs' ⊆ tcons κ κs →
+   Pκs [] →
+   Pκs [Vis κ] →
+   thas_trace_rel (λ κs, Pκs (Vis κ::κs)) κs →
+   thas_trace_rel Pκs κs'
+| TRel_ex (Pκs : _ → Prop) T f κs:
+   κs ⊆ tex T f →
+   Pκs [] →
+   (∀ x, thas_trace_rel Pκs (f x)) →
+   thas_trace_rel Pκs κs
+.
+
+Lemma thas_trace_rel_mono_l {EV} (Pκs1 Pκs2 : _ → Prop) (κs : trace EV) :
+  thas_trace_rel Pκs1 κs →
+  (∀ x, Pκs1 x → Pκs2 x) →
+  thas_trace_rel Pκs2 κs.
+Proof.
+  move => Ht. elim: Ht Pκs2.
+  - move => ?????? Hsub. apply: TRel_nil => //; by apply: Hsub.
+  - move => *. apply: TRel_cons; naive_solver.
+  - move => *. apply: TRel_ex; naive_solver.
+Qed.
+
+Lemma thas_trace_rel_mono_r {EV} Pκs (κs1 κs2 : trace EV) :
+  thas_trace_rel Pκs κs1 →
+  κs2 ⊆ κs1 →
+  thas_trace_rel Pκs κs2.
+Proof.
+  move => Ht. elim: Ht κs2.
+  - move => ???????. apply: TRel_nil => //. by etrans.
+  - move => *. apply: TRel_cons; [|done..]. by etrans.
+  - move => *. apply: TRel_ex; [|done..]. by etrans.
+Qed.
+
+Lemma thas_trace_rel_tnil {EV} Pκs (κs : trace EV) :
+  thas_trace_rel Pκs κs →
+  tnil ⊆ κs →
+  Pκs [] ∧ Pκs [Nb].
+Proof.
+  elim.
+  - done.
+  - move => ???? Hsub1 ???? Hsub2.
+    pose proof (transitivity Hsub2 Hsub1) as Ht. inversion Ht; simplify_K.
+  - move => ???? Hsub1 ??? Hsub2.
+    pose proof (transitivity Hsub2 Hsub1) as Ht. inversion Ht; simplify_K. naive_solver.
+Qed.
+
+Lemma thas_trace_rel_tcons {EV} Pκs (κs : trace EV) κs' κ :
+  thas_trace_rel Pκs κs →
+  tcons κ κs' ⊆ κs →
+  Pκs [Vis κ] ∧ thas_trace_rel (λ κs, Pκs (Vis κ :: κs)) κs'.
+Proof.
+  elim.
+  - move => ?? Hsub1 ?? Hsub2.
+    pose proof (transitivity Hsub2 Hsub1) as Ht. inversion Ht; simplify_K.
+  - move => ???? Hsub1 ???? Hsub2.
+    pose proof (transitivity Hsub2 Hsub1) as Ht. inversion Ht; simplify_K.
+    split; [done|]. by apply: thas_trace_rel_mono_r.
+  - move => ???? Hsub1 ??? Hsub2.
+    pose proof (transitivity Hsub2 Hsub1) as Ht. inversion Ht; simplify_K. naive_solver.
+Qed.
+
+Lemma thas_trace_rel_tall {EV} Pκs (κs : trace EV) T f :
+  thas_trace_rel Pκs κs →
+  tall T f ⊆ κs →
+  ∃ x, thas_trace_rel Pκs (f x).
+Proof.
+  elim.
+  - move => ?? Hsub1 ?? Hsub2.
+    pose proof (transitivity Hsub2 Hsub1) as Ht. inversion Ht; simplify_K. eexists _.
+    by apply: TRel_nil.
+  - move => ???? Hsub1???? Hsub2.
+    pose proof (transitivity Hsub2 Hsub1) as Ht. inversion Ht; simplify_K. eexists _.
+    by apply: TRel_cons.
+  - move => ???? Hsub1 ??? Hsub2.
+    pose proof (transitivity Hsub2 Hsub1) as Ht.
+    inversion Ht; simplify_K.
+    + naive_solver.
+    + eexists _. by apply: TRel_ex.
+Qed.
+
+Lemma thas_trace_rel_nil {EV} Pκs (κs : trace EV) :
+  thas_trace_rel Pκs κs →
+  Pκs [].
+Proof. inversion 1; by simplify_eq. Qed.
+
+Lemma shas_trace_thas_trace {EV} (m : module EV) σ Pσ (Pκs : _ → Prop):
+  σ ~{ m, Pκs }~>ₛ Pσ ↔ ∃ κs, thas_trace_rel Pκs κs ∧ σ ~{ m, κs }~>ₜ Pσ.
+Proof.
+  split.
+  - elim.
+    + move => ???? [??]. eexists tnil. split; [by constructor|]. by apply: TTraceEnd.
+    + move => ?? Pσ2 ? κ Hstep ? IH [??].
+      have [f Hf] := CHOICE IH.
+      eexists (tapp (option_trace κ) (tex _ f)).
+      split.
+      * destruct κ => /=.
+        -- apply: TRel_cons; [done..|]. apply: TRel_ex; [done..|] => -[??]. naive_solver.
+        -- apply: TRel_ex; [done..|] => -[??]. naive_solver.
+      * apply: TTraceStep; [done..| |done].
+        move => ??. apply: thas_trace_ex. naive_solver.
+  - move => [κs [Hκs Ht]].
+    elim: Ht Pκs Hκs.
+    + move => ???????. apply: STraceEnd; [done|].
+      by apply: thas_trace_rel_tnil.
+    + move => ??? κ ???? IH ?? Hrel.
+      move: (Hrel) => /thas_trace_rel_nil?.
+      apply: STraceStep; [done| |].
+      * move => ??. apply: IH; [done| ].
+        destruct κ => //; simplify_eq/=. 2: by apply: thas_trace_rel_mono_r.
+        efeed pose proof @thas_trace_rel_tcons as H; [done..|]. naive_solver.
+      * split; [done|]. destruct κ => //; simplify_eq/=.
+        efeed pose proof @thas_trace_rel_tcons as H; [done..|]. naive_solver.
+    + move => ?????? IH Hall ??.
+      have := thas_trace_rel_tall _ _ _ _ ltac:(done) ltac:(done).
+      naive_solver.
+      Unshelve. done.
+Qed.
+
+Lemma trefines_srefines {EV} (m1 m2 : mod_state EV):
+  trefines m1 m2 → srefines m1 m2.
+Proof.
+  move => [?]. constructor => ? /shas_trace_thas_trace[?[??]].
+  apply/shas_trace_thas_trace. naive_solver.
+Qed.
+(* Print Assumptions trefines_refines. *)
+
+Fixpoint trace_to_set {EV} (κs : trace EV) : list (event EV) → Prop :=
+  match κs with
+  | tnil => λ κs, κs = [] ∨ κs = [Nb]
+  | tcons κ κs => λ κs', κs' = [] ∨ ∃ κs'', κs' = Vis κ::κs'' ∧ trace_to_set κs κs''
+  | tex T f => λ κs, ∃ x, trace_to_set (f x) κs
+  | tall T f => λ κs, ∀ x, trace_to_set (f x) κs
+  end.
+
+(* The following cannot be provable since [refines m1 m2 → trefines m1 m2] does not hold. *)
+Lemma thas_trace_has_trace {EV} (m : module EV) σ Pσ κs:
+  σ ~{ m, κs }~>ₜ Pσ ↔ σ ~{ m, trace_to_set κs }~>ₛ Pσ.
+Proof.
+  rewrite shas_trace_thas_trace. split.
+  - move => ?. eexists _. split; [|done].
+    clear. elim: κs => /=.
+    + apply: TRel_nil; naive_solver.
+    + move => ???. apply: TRel_cons; [done|naive_solver| |].
+      * right. eexists _. split; [done|]. by apply: thas_trace_rel_nil.
+      * apply: thas_trace_rel_mono_l; [done|]. naive_solver.
+    + move => ?? IH.
+      apply: TRel_ex; [done| |]. admit.
+      move => ?. apply: thas_trace_rel_mono_l. done. naive_solver.
+    + move => ?? IH.
+      admit.
+  - move => [κs' [Hrel Ht]]. apply: thas_trace_mono; [done| |done]. clear Ht.
+    move: Hrel. move HPκs: (trace_to_set _) => Pκs Ht.
+    have : ∀ x, Pκs x → trace_to_set κs x by rewrite HPκs => ?.
+    elim: Ht κs {HPκs}.
+    + move => ???? Hnb κs Hsub. etrans; [done|].
+      move: Hnb => /Hsub /=. elim: κs {Hsub} => //=.
+      * naive_solver.
+      * move => ??? [??]. econstructor. naive_solver.
+      * move => ????. econstructor. naive_solver.
+    + move => ???????????. etrans; [done|].
+      admit.
+    + move => ??????????. etrans; [done|].
+      constructor. naive_solver.
+Abort.
+
+Lemma refines_not_trefines:
+  ¬ (∀ EV (m1 m2 : mod_state EV), srefines m1 m2 → trefines m1 m2).
+Proof.
+  move => Hr. apply: mod_ang_comm_not_refines. apply: Hr.
+  apply mod_ang_comm_equiv.
+Qed.
+
+(*** Equivalence between refines and dem_refines *)
+
+Inductive dem_trace_to_set {EV} : list (dem_event EV) → (list (event EV) → Prop) → Prop :=
+| DT2S_nil (Pκs : _ → Prop):
+    Pκs [] →
+    Pκs [Nb] →
+    dem_trace_to_set [] Pκs
+| DT2S_vis κ κs (Pκs : _ → Prop):
+    Pκs [] →
+    dem_trace_to_set κs (λ κs, Pκs (Vis κ::κs)) →
+    dem_trace_to_set (DVis κ :: κs) Pκs
+| DT2S_ub κs (Pκs : _ → Prop):
+    Pκs [] →
+    dem_trace_to_set (DUb :: κs) Pκs
+.
+
+Lemma dem_trace_to_set_nil {EV} (κs : list (dem_event EV)) Pκs:
+  dem_trace_to_set κs Pκs → Pκs [].
+Proof. inversion 1 => //; simplify_eq; naive_solver.  Qed.
+
+Lemma dem_trace_to_set_mono {EV} (κs : list (dem_event EV)) (Pκs Pκs' : _ → Prop):
+  dem_trace_to_set κs Pκs →
+  (∀ x, Pκs x → Pκs' x) →
+  dem_trace_to_set κs Pκs'.
+Proof.
+  move => Ht. elim: Ht Pκs'.
+  - move => ???? Hsub. constructor; by apply: Hsub.
+  - move => ????? IH ? Hsub. constructor. { by apply: Hsub. }
+    apply: IH => ??. by apply: Hsub.
+  - move => ???? Hsub. constructor. by apply: Hsub.
+Qed.
+
+Lemma has_trace_dem_has_trace {EV} (m : dem_module EV) σ Pσ Pκs:
+  σ ~{ m, Pκs }~>ₛ Pσ ↔ ∃ κs, dem_trace_to_set κs Pκs ∧ σ ~{ m, κs }~>ₘ Pσ.
+Proof.
+  split.
+  - elim.
+    + move => ???? [??]. eexists [] => /=. split;[by constructor|]. by constructor.
+    + move => ???? κ Hstep _ IH ?.
+      inversion Hstep; simplify_eq.
+      * have [κs [Hsub ?]]:= IH _ ltac:(done).
+        eexists (option_list (DVis <$> _) ++ κs).
+        split. 2: by apply: DTraceStep.
+        destruct κ => //=. constructor => //. naive_solver.
+      * eexists [DUb]. split; [constructor| by apply: DTraceUb]. naive_solver.
+  - move => [κs [HP Ht]].
+    elim: Ht Pκs HP.
+    + move => ???? Ht. inversion Ht; simplify_eq. by constructor.
+    + move => σ1 σ2 Pσ3 κ κs' Hstep _ IH Pκs Ht.
+      apply: STraceStep. { by constructor. } 2: {
+        move: (Ht) => /dem_trace_to_set_nil ?.
+        destruct κ => //. inversion Ht; simplify_eq/=.
+        split; [done|]. move: H3 => /dem_trace_to_set_nil. done.
+       }
+      move => ? ->. apply: IH.
+      destruct κ => //; simplify_eq/=. by inversion Ht; simplify_eq.
+    + move => ????? Ht. apply: STraceStep; [ by constructor | done | ].
+      split; by apply: dem_trace_to_set_nil.
+Qed.
+
+
+Fixpoint events_to_set {EV} (κs : list (dem_event EV)) : list (event EV) → Prop :=
+  match κs with
+  | [] => λ κs'', κs'' = []  ∨ κs'' = [Nb]
+  | DUb::_ => λ κs'', κs'' = []  ∨ κs'' = [Ub]
+  | DVis κ::κs' => λ κs'', (κs'' = [])
+      ∨ ∃ κs''', κs'' = Vis κ::κs''' ∧ events_to_set κs' κs'''
+  end.
+
+(* Compute events_to_set [Vis 1]. *)
+(* Compute events_to_set [Vis 1; Ub]. *)
+(* Compute events_to_set [Ub]. *)
+
+Lemma events_to_set_nil {EV} (κs : list (dem_event EV)) :
+  events_to_set κs [].
+Proof. destruct κs as [|[|]] => //; naive_solver. Qed.
+
+Lemma dem_trace_to_set_events {EV} (κs : list (dem_event EV)) :
+  dem_trace_to_set κs (events_to_set κs).
+Proof.
+  elim: κs. 1: constructor; naive_solver.
+  move => [|κ] κs IH /=. 1: constructor; by left.
+  constructor.
+  - by left.
+  - apply: dem_trace_to_set_mono; [done|] => ??. naive_solver.
+Qed.
+
+Lemma dem_trace_to_set_inj {EV} (κs1 κs2 : list (dem_event EV)):
+  dem_trace_to_set κs2 (events_to_set κs1) →
+  κs1 = κs2 ∨ ∃ κs, κs ++ [DUb] `prefix_of` κs2 ∧ κs `prefix_of` κs1.
+Proof.
+  elim: κs2 κs1 => [|[|κ2] κs2] /=.
+  - move => [|[|κ] κs] Hdem.
+    + naive_solver.
+    + inversion Hdem; simplify_eq/=. naive_solver.
+    + inversion Hdem; simplify_eq/=.
+      have := events_to_set_nil κs. naive_solver.
+  - move => IH κs1 /= Hdem. right. eexists [].
+    split; [apply: prefix_cons|]; apply: prefix_nil.
+  - move => IH [|[|κ] κs] /=; inversion 1; simplify_eq/=.
+    + move: H4 => /dem_trace_to_set_nil. naive_solver.
+    + move: H4 => /dem_trace_to_set_nil. naive_solver.
+    + move: (H4) => /dem_trace_to_set_nil [//|[?[??]]]; simplify_eq.
+      have [| |]:= IH κs.
+      -- apply: dem_trace_to_set_mono; [done|] => ??. naive_solver.
+      -- naive_solver.
+      -- move => [κs1 [??]]. right.
+         eexists (_:: _) => /=. split; by apply: prefix_cons.
+Qed.
+
+Lemma dem_has_trace_has_trace {EV} (m : dem_module EV) σ Pσ κs:
+  σ ~{ m, κs }~>ₘ Pσ ↔ σ ~{ m, events_to_set κs}~>ₛ Pσ.
+Proof.
+  rewrite has_trace_dem_has_trace.
+  split.
+  - move => ?. eexists _. split; [|done]. apply: dem_trace_to_set_events.
+  - move => [κs2[/dem_trace_to_set_inj[->//|[?[[?->][?->]]]]]].
+    move => /dem_has_trace_app_inv/dem_has_trace_ub_app_inv ?.
+    by apply: dem_has_trace_trans.
+Qed.
+
+Lemma dem_refines_refines {EV} (m1 m2 : dem_mod_state EV):
+  dem_refines m1 m2 → srefines m1 m2.
+Proof.
+  move => [?]. constructor => ? /has_trace_dem_has_trace?.
+  apply/has_trace_dem_has_trace. naive_solver.
+Qed.
+
+Lemma refines_dem_refines {EV} (m1 m2 : dem_mod_state EV):
+  srefines m1 m2 → dem_refines m1 m2.
+Proof.
+  move => [?]. constructor => ?.
+  move => /dem_has_trace_has_trace?.
+  apply/dem_has_trace_has_trace. naive_solver.
+Qed.
